cava/Cava/Arrow/ExprSyntax.v
@@ -10,88 +10,86 @@ Import ListNotations.
 Set Implicit Arguments.
 Set Asymmetric Patterns.
 
-Section vars.
-  Definition natvar : Kind -> Type := fun _ => nat.
-  Definition unitvar : Kind -> Type := fun _ => unit.
+Definition natvar : Kind -> Type := fun _ => nat.
+Definition unitvar : Kind -> Type := fun _ => unit.
 
-  Definition extended_prim_input p :=
-    match p with
-    | P0 _ _ => Unit
-    | P1 x _ _ => Tuple x Unit
-    | P2 x y z _ => Tuple x (Tuple y Unit)
-    end.
+Definition extended_prim_input p :=
+  match p with
+  | P0 _ _ => Unit
+  | P1 x _ _ => Tuple x Unit
+  | P2 x y z _ => Tuple x (Tuple y Unit)
+  end.
 
-  Record Module ( body_ty : Type ) := mkModule
-    { module_name : string
-    ; module_body : body_ty
-    }.
+Record Module ( body_ty : Type ) := mkModule
+  { module_name : string
+  (* ; module_args : _ *)
+  ; module_body : body_ty
+  }.
 
-  Definition module_map_body {A B} (m: Module A) (f: A -> B): Module B :=
-    match m with
-    | mkModule name body => mkModule name (f body)
-    end.
+Definition module_map_body {A B} (m: Module A) (f: A -> B): Module B :=
+  match m with
+  | mkModule name body => mkModule name (f body)
+  end.
 
-  Section Vars.
-    Variable (var: Kind -> Type).
+Section Vars.
+  Inductive kappa {var: Kind -> Type}: Kind -> Kind -> Type :=
+  | Var : forall {x},     var x -> kappa Unit x
+  | Abs : forall {x y z}, (var x -> kappa y z) -> kappa (Tuple x y) z
+  | App : forall {x y z}, kappa (Tuple x y) z -> kappa Unit x -> kappa y z
+  | Comp: forall {x y z}, kappa y z -> kappa x y -> kappa x z
+  | Comp1: forall {x y z}, kappa y z -> kappa x (remove_rightmost_unit y) -> kappa x z
+  | Delay: forall {x}, kappa (Tuple x Unit) x
+  | Primitive : forall prim, kappa (extended_prim_input prim) (primitive_output prim)
+  | Let: forall {x y z}, kappa Unit x -> (var x -> kappa y z) -> kappa y z
+  | LetRec : forall {x y z}, (var x -> kappa Unit x) -> (var x -> kappa y z) -> kappa y z
+  | Id : forall {x}, kappa x x
+  | Typecast : forall x y, kappa (Tuple x Unit) y
+  | CallModule: forall {x y}, Module (forall var, kappa (var:=var) x y) -> kappa x y
+  .
+End Vars.
+Arguments kappa : clear implicits.
 
-    Inductive kappa : Kind -> Kind -> Type :=
-    | Var : forall {x},     var x -> kappa Unit x
-    | Abs : forall {x y z}, (var x -> kappa y z) -> kappa (Tuple x y) z
-    | App : forall {x y z}, kappa (Tuple x y) z -> kappa Unit x -> kappa y z
-    | Comp: forall {x y z}, kappa y z -> kappa x y -> kappa x z
-    | Comp1: forall {x y z}, kappa y z -> kappa x (remove_rightmost_unit y) -> kappa x z
-    | Delay: forall {x}, kappa (Tuple x Unit) x
-    | Primitive : forall prim, kappa (extended_prim_input prim) (primitive_output prim)
-    | Let: forall {x y z}, kappa Unit x -> (var x -> kappa y z) -> kappa y z
-    | LetRec : forall {x y z}, (var x -> kappa Unit x) -> (var x -> kappa y z) -> kappa y z
-    | Id : forall {x}, kappa x x
-    | Typecast : forall x y, kappa (Tuple x Unit) y
-    | RemoveContext: forall {x y}, kappa x y -> kappa x y
-    | CallModule: forall {x y}, Module (kappa x y) -> kappa x y
-    .
-  End Vars.
+Fixpoint reverse_nth {A} (l: list A) (n: nat) {struct l}: option A :=
+  match l with
+  | [] => None
+  | x :: xs =>
+    match eq_nat_dec n (length xs) with
+    | left _ => Some x
+    | right Hneq => reverse_nth xs n
+    end
+  end.
 
-  Fixpoint reverse_nth {A} (l: list A) (n: nat) {struct l}: option A :=
-    match l with
-    | [] => None
-    | x :: xs =>
-      match eq_nat_dec n (length xs) with
-      | left _ => Some x
-      | right Hneq => reverse_nth xs n
-      end
-    end.
+Notation ok_lookup := (fun (l: list _) (n: nat) (ty: _) => reverse_nth l n = Some ty).
 
-  Notation ok_lookup := (fun (l: list _) (n: nat) (ty: _) => reverse_nth l n = Some ty).
+Fixpoint wf_phoas_context {i o}
+  (ctxt: list Kind)
+  (expr: kappa natvar i o) {struct expr}
+  : Prop :=
+  match expr with
+  | Var _ n  => ok_lookup ctxt n o
+  | Abs x _ _ f => wf_phoas_context (x :: ctxt) (f (length ctxt))
+  | App _ _ _ e1 e2 => wf_phoas_context ctxt e1 /\ wf_phoas_context ctxt e2
+  | Comp _ _ _ e1 e2 => wf_phoas_context ctxt e1 /\ wf_phoas_context ctxt e2
+  | Comp1 _ _ _ e1 e2 => wf_phoas_context ctxt e1 /\ wf_phoas_context ctxt e2
+  | Delay _ => True
+  | Primitive _ => True
+  | Id _ => True
+  | Typecast x y => True
+  | Let x _ _ v f => wf_phoas_context (x :: ctxt) (f (length ctxt)) /\ wf_phoas_context ctxt v
+  | LetRec x _ _ v f => wf_phoas_context (x :: ctxt) (v (length ctxt)) /\ wf_phoas_context (x :: ctxt) (f (length ctxt))
+  | CallModule _ _ (mkModule _ m) => wf_phoas_context [] (m natvar)
+  end.
 
-  Fixpoint wf_phoas_context {i o}
-    (ctxt: list Kind)
-    (expr: kappa natvar i o) {struct expr}
-    : Prop :=
-    match expr with
-    | Var _ n  => ok_lookup ctxt n o
-    | Abs x _ _ f => wf_phoas_context (x :: ctxt) (f (length ctxt))
-    | App _ _ _ e1 e2 => wf_phoas_context ctxt e1 /\ wf_phoas_context ctxt e2
-    | Comp _ _ _ e1 e2 => wf_phoas_context ctxt e1 /\ wf_phoas_context ctxt e2
-    | Comp1 _ _ _ e1 e2 => wf_phoas_context ctxt e1 /\ wf_phoas_context ctxt e2
-    | Delay _ => True
-    | Primitive _ => True
-    | Id _ => True
-    | Typecast x y => True
-    | Let x _ _ v f => wf_phoas_context (x :: ctxt) (f (length ctxt)) /\ wf_phoas_context ctxt v
-    | LetRec x _ _ v f => wf_phoas_context (x :: ctxt) (v (length ctxt)) /\ wf_phoas_context (x :: ctxt) (f (length ctxt))
-    | RemoveContext _ _ f => wf_phoas_context [] f
-    | CallModule _ _ (mkModule _ m) => wf_phoas_context [] m
-    end.
+Definition Kappa i o := forall var, kappa var i o.
 
-  Definition Kappa i o := forall var, kappa var i o.
+Definition module_instantiate_var {var x y} (m: Module (Kappa x y)): Module (kappa var x y) :=
+  module_map_body m (fun e => e var).
 
-  Definition module_instantiate_var {var x y} (m: Module (Kappa x y)): Module (kappa var x y) :=
-    module_map_body m (fun e => e var).
-  Definition module_to_expr {x y} (e: Module (Kappa x y)): Kappa x y :=
-    fun var => CallModule (module_instantiate_var e).
+Definition ModuleK i o := Module (Kappa i o).
 
-  Coercion module_to_expr: Module >-> Kappa.
-End vars.
+Definition module_to_expr {x y} (e: ModuleK x y): Kappa x y := module_body e.
+
+Coercion module_to_expr: ModuleK >-> Kappa.
 
 Arguments Var {var _}.
 Arguments Abs {var _ _ _}.
@@ -103,7 +101,6 @@ Arguments Primitive {var}.
 Arguments LetRec {var _ _ _}.
 Arguments Id {var _}.
 Arguments Typecast {var}.
-Arguments RemoveContext {var _ _}.
 Arguments CallModule {var _ _}.
 
 Instance KappaCat : Category Kind := {
