silveroak-opentitan/aes/Arrow/pkg.v
@@ -22,8 +22,10 @@ Import VectorNotations.
 Import KappaNotation.
 Open Scope kind_scope.
 
+Local Notation instantiate f := (CallModule f).
+
 Notation "|^ x" :=
-  (App (RemoveContext (foldr1 <[\a b => xor a b]> _)) x)
+  (App (instantiate (foldr1 <[\a b => xor a b]>)) x)
   (in custom expr at level 5, no associativity) : kappa_scope.
 Notation "x && y" :=
   (App (App (Primitive (P2 And)) x) y)
@@ -32,16 +34,16 @@ Notation "x || y" :=
   (App (App (Primitive (P2 And)) x) y)
   (in custom expr at level 6, left associativity) : kappa_scope.
 Notation "x & y" :=
-  (App (App (RemoveContext (bitwise <[and]>  _)) x) y)
+  (App (App (instantiate (bitwise <[and]>)) x) y)
   (in custom expr at level 6, left associativity) : kappa_scope.
 Notation "x ^ y" :=
-  (App (App (RemoveContext (bitwise <[xor]> _)) x) y)
+  (App (App (instantiate (bitwise <[xor]>)) x) y)
     (in custom expr at level 6, left associativity) : kappa_scope.
 Notation "'if' i 'then' t 'else' e" :=
-  (App (App (App (RemoveContext (mux_item _)) i) t) e)
+  (App (App (App (instantiate mux_item) i) t) e)
   (in custom expr at level 5, left associativity) : kappa_scope.
 Notation "x == y" :=
-  (App (App (RemoveContext (equality _)) x) y)
+  (App (App (instantiate equality) x) y)
   (in custom expr at level 6, left associativity) : kappa_scope.
 
 Inductive SboxImpl :=
